cvc5/Basic.lean
@@ -1,0 +1,955 @@
+/-
+Copyright (c) 2023-2024 by the authors listed in the file AUTHORS and their
+institutional affiliations. All rights reserved.
+Released under Apache 2.0 license as described in the file LICENSE.
+Authors: Abdalrhman Mohamed, Adrien Champion
+-/
+
+import Lean.Elab.Command
+
+import cvc5.Kind
+import cvc5.ProofRule
+import cvc5.SkolemId
+import cvc5.Types
+
+
+
+/-! # Helpers and basic definitions -/
+namespace cvc5
+
+
+
+/-! ## Errors and environment -/
+
+
+
+/-- A kind of error. -/
+inductive Error.Kind
+/-- A plain error. -/
+| error
+/-- A recoverable error. -/
+| recoverable
+/-- Unsupported feature. -/
+| unsupported
+/-- Bad option error. -/
+| option
+deriving Repr
+
+/-- Error type. -/
+structure Error where mk' ::
+  /-- The error message. -/
+  msg : String
+  /-- The error kind. -/
+  (kind : Error.Kind := .error)
+deriving Repr
+
+namespace Error
+
+/-- Error constructor. -/
+def mk (msg : String) (kind : Error.Kind := .error) : Error := {msg, kind}
+
+@[inherit_doc Kind.recoverable]
+def recoverable (msg : String) : Error := mk msg .recoverable
+@[inherit_doc Kind.unsupported]
+def unsupported (msg : String) : Error := mk msg .unsupported
+@[inherit_doc Kind.option]
+def option (msg : String) : Error := mk msg .option
+
+namespace Kind
+
+/-- Error prefix. -/
+def pref : Kind → String
+  | error => ""
+  | recoverable => "[recoverable] "
+  | unsupported => "[unsupported] "
+  | option => "[option] "
+
+/-- String representation. -/
+protected def toString (k : Kind) : String := s!"{k.pref}error"
+
+instance : ToString Kind := ⟨Kind.toString⟩
+
+end Kind
+
+/-- String representation. -/
+protected def toString (e : Error) : String :=
+  s!"{e.kind.pref}{e.msg}"
+
+instance : ToString Error := ⟨Error.toString⟩
+
+/-- Panics on errors. -/
+def unwrap! [Inhabited α] : Except Error α → α
+  | .ok a => a
+  | .error e => panic! e.toString
+
+/-! ### Exports for the C++ layer -/
+
+section ffi_except_constructors
+
+/-- Only used by FFI to inject values. -/
+@[export generic_except_ok]
+private def mkExceptOk {α : Type} : α → Except Error α :=
+  .ok
+
+/-- Only used by FFI to inject values. -/
+@[export except_ok_bool]
+private def mkExceptOkBool : Bool → Except Error Bool :=
+  .ok
+
+/-- Only used by FFI to inject values. -/
+@[export except_ok_u32]
+private def mkExceptOkU32 : UInt32 → Except Error UInt32 :=
+  .ok
+
+/-- Only used by FFI to inject values. -/
+@[export except_ok_u16]
+private def mkExceptOkU16 : UInt16 → Except Error UInt16 :=
+  .ok
+
+/-- Only used by FFI to inject values. -/
+@[export except_ok_u8]
+private def mkExceptOkU8 : UInt8 → Except Error UInt8 :=
+  .ok
+
+/-- Only used by FFI to inject errors. -/
+@[export except_err]
+private def mkExceptErr {α : Type} : String → Except Error α := .error ∘ mk
+
+end ffi_except_constructors
+
+end Error
+
+
+
+/-- Cvc5 environment monad transformer.
+
+Most monadic functions in this API use the non-transformer monad `cvc5.Env`, where `m := BaseIO`.
+
+When using an `EnvT m α`, do make sure `m` is such that `MonadLiftT BaseIO m` which gives
+`MonadLiftT Env (EnvT m)`.
+-/
+def EnvT (m : Type → Type) (α : Type) : Type := ExceptT Error m α
+
+/-- Cvc5 environment (`EnvT`) in `BaseIO`. -/
+abbrev Env (α : Type) : Type := EnvT BaseIO α
+
+namespace Env
+
+/-! ### Monad-related instances -/
+section monad_instances variable [Monad m]
+
+/-- Provides an instance by unfolding `EnvT` and running inference. -/
+private def infer {α : Sort u} (a : α := by unfold EnvT ; infer_instance) : α := a
+
+instance : Monad (EnvT m) := infer
+example : Monad Env := inferInstance
+
+instance : MonadExceptOf Error (EnvT m) := infer
+example : MonadExceptOf Error Env := inferInstance
+
+instance : MonadLift m (EnvT m) := infer
+example : MonadLift BaseIO Env := inferInstance
+
+instance : MonadLift (Except Error) (EnvT m) := infer
+
+instance [L : MonadLiftT BaseIO m] : MonadLift Env (EnvT m) where
+  monadLift code := return ← L.monadLift code
+example : MonadLift Env (EnvT IO) := inferInstance
+
+instance [MonadLiftT BaseIO m] : MonadLift IO (EnvT m) where
+  monadLift code := do
+    match ← code.toBaseIO with
+    | .ok a => return a
+    | .error e => Error.mk e.toString |> throw
+example [MonadLiftT BaseIO m] : MonadLiftT BaseIO (EnvT m) := inferInstance
+example : MonadLift IO Env := inferInstance
+end monad_instances
+
+/-! ### Exports for the C++ layer -/
+section cpp_exports
+
+@[export env_pure]
+private def env_pure (a : α) : Env α := return a
+
+@[export env_bool]
+private def env_bool (b : Bool) : Env Bool := return b
+
+@[export env_uint64]
+private def env_uint64 (u : UInt64) : Env UInt64 := return u
+
+@[export env_throw]
+private def env_throw (e : Error) : Env α := throw e
+
+@[export env_throw_string]
+private def env_throw_string (msg : String) : Env α := Error.mk msg |> throw
+
+end cpp_exports
+
+/-! ### Runners -/
+section runners variable [Monad m]
+
+/-- Runs `EnvT` code. -/
+def run [MonadLiftT BaseIO m] : EnvT m α → m (Except Error α) := id
+
+/-- Runs `EnvT` code in `IO`. -/
+def runIO [MonadLiftT m IO] (code : EnvT m α) : IO α := do
+  match ← code.run with
+  | .ok a => return a
+  | .error e => IO.userError e.toString |> throw
+
+end runners
+
+end Env
+
+@[inherit_doc Env.run]
+protected abbrev EnvT.run := @Env.run
+
+@[inherit_doc Env.run]
+protected abbrev run := @Env.run
+
+
+
+/-! ## Basic export for the C++ layer -/
+
+
+
+namespace CppExports
+
+@[export prod_mk]
+private def mkProd := @Prod.mk
+
+end CppExports
+
+
+
+/-! ## DSL for definition  DRY -/
+section defsMacro
+
+
+
+open Lean
+open Elab
+open Command (CommandElab CommandElabM)
+
+declare_syntax_cat externKw
+
+declare_syntax_cat defsItem
+declare_syntax_cat defsItemHead
+declare_syntax_cat defsItemTail!?
+declare_syntax_cat defsItemTail
+
+declare_syntax_cat defsMod
+
+/-- Arity of an expression.
+
+Stolen from [batteries].
+
+[batteries]: https://leanprover-community.github.io/mathlib4_docs/Batteries/Lean/Expr.html#Lean.Expr.forallArity
+-/
+def forallArity : Expr → Nat
+  | .mdata _ b => forallArity b
+  | .forallE _ _ body _ => 1 + forallArity body
+  | _ => 0
+
+syntax "?" : defsMod
+syntax "!" : defsMod
+syntax "!?" : defsMod
+syntax "?!" : defsMod
+
+scoped syntax (name := defsItemStxHead)
+  declModifiers
+  ("@[" "force" str "]")?
+  "def " defsMod ? ident
+: defsItemHead
+
+scoped syntax (name := defsItemStxTail!?)
+  withPosition(ppLine "with!? "
+    group(
+      colGt
+      docComment ?
+      ident
+    )*
+  )
+: defsItemTail!?
+
+scoped syntax (name := defsItemStxTail)
+  withPosition(ppLine "with "
+    group(
+      colGt
+      docComment ?
+      declId optDeclSig ":= " withPosition(group(colGe term))
+    )*
+  )
+: defsItemTail
+
+scoped syntax (name := defsItemStx)
+  defsItemHead
+  declSig
+  (defsItemTail!?)?
+  (defsItemTail)?
+: defsItem
+
+unsafe def elabDefsItem
+  (pref : String) (forceMods : Option (TSyntax `defsMod))
+: CommandElab
+| `(defsItem|
+    $mods:declModifiers
+    $[ @[ force $forcedName ] ]?
+    def $ident:ident $identSig:declSig
+    $[ with!? $[
+        $[$autoDoc]?
+        $autoId
+    ]* ]?
+    $[ with $[
+        $[$subDoc]?
+        $subId $subSig := $subDef
+    ]* ]?
+) => do
+  if let some defMods := forceMods then
+    let stx ← `(defsItem|
+$mods:declModifiers
+$[ @[ force $forcedName ] ]?
+def $defMods $ident:ident $identSig:declSig
+$[ with!? $[
+    $[$autoDoc]?
+    $autoId
+]* ]?
+$[ with $[
+    $[$subDoc]?
+    $subId $subSig := $subDef
+]* ]?
+    )
+    return ← elabDefsItem pref none stx
+
+  let externName :=
+    let id :=
+      if let some forcedName := forcedName then
+        forcedName.getString
+      else
+        ident.getId.toString
+    pref ++ "_" ++ id |> Syntax.mkStrLit
+  -- println! "extern name := `{externName}`"
+  let mods ←
+    match mods with
+    | `(Parser.Command.declModifiersT|
+      $[$doc:docComment]? $[@[ $[ $attrs ],* ]]? $[$vis]? $[$isNc]? $[$isUnsafe]? $[$opt]?
+    ) => do
+      let ext ← `(Parser.Term.attrInstance| extern $externName:str)
+      let attrs := attrs.getD #[] |>.push ext
+      `(Parser.Command.declModifiersT|
+        $[$doc:docComment]? @[ $[$attrs],* ] $[$vis]? $[$isNc]? $[$isUnsafe]? $[$opt]?
+      )
+    | _ => throwUnsupportedSyntax
+  let mainDef ←`(
+    set_option linter.unusedVariables false in
+    $(⟨mods⟩):declModifiers
+    opaque $ident:declId $identSig
+  )
+  Command.elabCommand mainDef
+
+  let fullName :=
+    Lean.Name.mkSimple ident.getId.toString
+    |> (← Elab.liftMacroM Macro.getCurrNamespace).append
+  let fullIdent := Lean.mkIdent fullName
+
+  let define doc? id sig? (body : Syntax.Term) : CommandElabM _ := do
+    if let some doc := doc? then
+      `(command|
+        $doc:docComment
+        def $id:declId $sig?:optDeclSig := $body
+      )
+    else
+      `(command|
+        @[inherit_doc $fullIdent]
+        def $id:declId $sig?:optDeclSig := $body
+      )
+
+  if let (some autoDoc?, some autoId) := (autoDoc, autoId) then
+    let env ← getEnv
+    let arity ←
+      if let some (.opaqueInfo i) := env.find? fullName then
+        pure (forallArity i.type)
+      else
+        throwError s!"failed to retrieve arity of (opaque) function `{ident}`"
+
+    let mut args := Array.empty
+    for i in [0:arity] do
+      let arg := Lean.Name.mkSimple s!"v{i}" |> Lean.mkIdent
+      args := args.push arg
+    let funCall : TSyntax `term ← `(term| ( $fullIdent $[ $args ]* ))
+
+    for (autoDoc?, autoId) in autoDoc?.zip autoId do
+      let id : String := autoId.getId.toString
+      let body ←
+        if id.endsWith "!" then
+          let unwrapName := Lean.Name.mkStr3 "cvc5" "Error" "unwrap!" |> Lean.mkIdent
+          `(fun $[$args]* => $funCall |> $unwrapName)
+        else if id.endsWith "?" then
+          `(fun $[$args]* => $funCall |> Except.toOption)
+        else
+          throwError s!"unexpected auto function name `{id}`: expected `<ident>!` or `<ident>?`"
+      let cmd ← define autoDoc? autoId (← `(optDeclSig|)) body
+      Command.elabCommand cmd
+
+  if let
+    (some subDoc?, some subId, some subSig, some subDef)
+    := (subDoc, subId, subSig, subDef)
+  then
+    let all := subDoc?.zip subId |>.zip subSig |>.zip subDef
+    for (((subDoc?, subId), subSig), subDef) in all do
+      Command.elabCommand
+        (← define subDoc? subId subSig subDef)
+| `(defsItem|
+    $mods:declModifiers
+    $[ @[ force $forcedName ] ]?
+    def $defsMod $ident:ident $identSig:declSig
+    $[ with $[
+        $[$subDoc]?
+        $subId $subSig := $subDef
+    ]* ]?
+) => do
+  let name := ident.getId
+  let identOpt _ := name.appendAfter "?" |> Lean.mkIdent
+  let identPanic _ := name.appendAfter "!" |> Lean.mkIdent
+  let auto : Array Ident ←
+    match defsMod with
+    | `(defsMod| ?) => pure #[identOpt ()]
+    | `(defsMod| !) => pure #[identPanic ()]
+    | `(defsMod| ?!)
+    | `(defsMod| !?) => pure #[identOpt (), identPanic ()]
+    | _ => throwUnsupportedSyntax
+  let stx ← `(defsItemStx|
+    $mods:declModifiers
+    $[ @[ force $forcedName ] ]?
+    def $ident:ident $identSig:declSig
+    with!? $[ $auto:ident ]*
+    $[ with $[
+        $[ $subDoc:docComment ]?
+        $subId:declId $subSig:optDeclSig := $subDef:term
+    ]* ]?
+  )
+  elabDefsItem pref none stx
+| _ => throwUnsupportedSyntax
+
+/-- Defines similar functions realized by `extern`.
+
+```
+extern! in "prefix"
+  /-- Create a Boolean constant.
+
+  - `b`: The Boolean constant.
+
+  Will create an opaque definition with `[@extern extStr]` where
+  `extStr = "prefix" ++ "_" ++ "myFunction"`.
+  -/
+  def myFunction : Term → Except Error Op
+  with!?
+    endsWithBang!
+    endWithQuestion?
+  with
+    myOtherFunction : Term → Op :=
+      Error.unwrap! ∘ myFunction
+    /-- Optional function docstring: if none, inherit from the main function. -/
+    yetAnotherFunction : Term → Option Op :=
+      Except.toOption ∘ myFunction
+```
+
+- `in "prefix"` is optional; if none, then the prefix will be the (last component of the) name of
+  the current namespace with the first letter lowercased. Fails if the current namespace has no
+  components.
+
+- `with ...`: takes a sequence of identifiers, each generate a function that
+  - unwraps the result if `!`-ended, which generates code similar to `myOtherFunction` above;
+  - turns a result into an option if `?`-ended, which generates code similar to `yetAnotherFunction`
+    above;
+  - fails otherwise.
+
+  The `with ...` syntax is currently only compatible with external functions that produce `Except
+  Error α` values.
+
+- Supports `declModifiers` on the main (`def`) function `myFunction` such as `private`.
+- Accepts a list of external (`def`) functions, each with its `with` clauses.
+
+This macro can generate optional (`?`) and panic (`!`) wrappers even more automatically.
+
+```
+extern! "prefix"
+  /-- Create a Boolean constant.
+
+  - `b`: The Boolean constant.
+
+  Will create an opaque definition with `[@extern extStr]` where
+  `extStr = "prefix" ++ "_" ++ "myFunction"`.
+  -/
+  def !? myFunction : Term → Except Error Op
+  with
+    myOtherFunction : Term → Op :=
+      myFunction!
+    /-- Optional function docstring: if none, inherit from the main function. -/
+    yetAnotherFunction : Term → Option Op :=
+      myFunction?
+```
+
+Notice the `!?` between `def` and `myFunction`. This generates `myFunction!` and `myFunction?` which
+respectively panic-unwrap errors and turn the `Except` into an `Option`. In other words, it is the
+same as (and internally turned into) a `with!? myFunction! myFunction?` clause using the first
+syntax above.
+
+Besides `!?`, the following are also supported:
+- `?!`: same behavior as `!?`;
+- `!`: only generate the panic unwrapper;
+- `?`: only generate the `Option` unwrapper.
+-/
+scoped syntax (name := multidefs)
+  withPosition("external! " ("in " str)? ppLine group(colGt defsItem)+)
+: command
+
+@[inherit_doc multidefs, command_elab multidefs]
+unsafe def multidefsImpl : CommandElab
+| `(command|
+  external! $[in $pref:str]? $[$defsItems]*
+) => do
+  let ns ← getCurrNamespace
+  let pref ←
+    if let some pref := pref then
+      pure pref.getString
+    else
+      -- println! "componentsRev for {ns.toString}"
+      -- for c in ns.componentsRev do
+      --   println! "- {c.toString}"
+      if let super::_ := ns.componentsRev then
+        let mut super := super.toString
+        if 0 < super.length then
+          super := String.Pos.Raw.get super 0 |>.toLower |> String.Pos.Raw.set super 0
+        -- println! "-> `{super}`"
+        pure super
+      else
+        throwError "failed to retrieve current workspace, please provide an explicit prefix"
+  for defsItem in defsItems do
+    elabDefsItem pref none defsItem
+| _ => throwUnsupportedSyntax
+
+scoped syntax (name := externkw)
+  ("extern_def " <|> "extern_def! " <|> "extern_def? " <|> "extern_def!? " <|> "extern_def?! ")
+: externKw
+
+/-- Defines an external, opaque function with optional helpers.
+
+```
+/-- Some documentation. -/
+extern_def!? in "prefix" myFunction : Term → Except Error Op
+```
+
+Generates an opaque definition
+
+```
+/-- Some documentation. -/
+@[extern "prefix_myFunction"]
+def myFunction : Term → Except Error Op
+```
+
+- `in "prefix"` is optional, uses the current namespace with first letter lowercased if none.
+
+- `extern_def!?` also defines `myFunction! : Term → Op` and `myFunction? : Term → Option Op` in
+  terms of `myFunction`.
+
+  Other variants exist:
+  - `extern_def?!`: same as `extern_def!?`;
+  - `extern_def?`: only defines `myFunction?`;
+  - `extern_def!`: only defines `myFunction!`;
+  - `extern_def`: defines nothing besides `myFunction`.
+-/
+scoped syntax (name := externdef)
+  declModifiers
+  withPosition(
+    externKw
+    ("in " str)?
+    ident declSig (defsItemTail)?
+  )
+: command
+
+@[inherit_doc externdef, command_elab externdef]
+unsafe def externdefImpl : CommandElab
+| `(command|
+  $mods:declModifiers
+  $externKw $[in $path:str]? $ident $sig $[$tail]?
+) => do
+  let defMod ←
+    match externKw with
+    | `(externKw| extern_def) => pure none
+    | `(externKw| extern_def!) => `(defsMod| !)
+    | `(externKw| extern_def?) => `(defsMod| ?)
+    | `(externKw| extern_def!?) => `(defsMod| !?)
+    | `(externKw| extern_def?!) => `(defsMod| ?!)
+    | _ => throwUnsupportedSyntax
+  let stx ← `(
+    external! $[in $path]?
+      $mods:declModifiers
+      def $[$defMod]? $ident $sig $[$tail:defsItemTail]?
+  )
+  Command.elabCommand stx
+| _ => throwUnsupportedSyntax
+
+end defsMacro
+
+
+
+/-! ## Definitions over auto-generated types -/
+
+
+
+namespace Kind
+
+/-- Produces a string representation. -/
+protected extern_def toString : Kind → String
+instance : ToString Kind := ⟨Kind.toString⟩
+
+/-- Produces a hash. -/
+extern_def hash : Kind → UInt64
+instance : Hashable Kind := ⟨Kind.hash⟩
+
+end Kind
+
+
+
+namespace SortKind
+
+/-- Produces a string representation. -/
+protected extern_def toString : SortKind → String
+instance : ToString SortKind := ⟨SortKind.toString⟩
+
+/-- Produces a hash. -/
+extern_def hash : SortKind → UInt64
+instance : Hashable SortKind := ⟨SortKind.hash⟩
+
+end SortKind
+
+
+
+namespace ProofRule
+
+/-- Produces a string representation. -/
+protected extern_def toString : ProofRule → String
+instance : ToString ProofRule := ⟨ProofRule.toString⟩
+
+/-- Produces a hash. -/
+extern_def hash : ProofRule → UInt64
+instance : Hashable ProofRule := ⟨ProofRule.hash⟩
+
+end ProofRule
+
+
+
+namespace SkolemId
+
+/-- Produces a string representation. -/
+protected extern_def toString : SkolemId → String
+instance : ToString SkolemId := ⟨SkolemId.toString⟩
+
+/-- Produces a hash. -/
+extern_def hash : SkolemId → UInt64
+instance : Hashable SkolemId := ⟨SkolemId.hash⟩
+
+end SkolemId
+
+
+
+namespace ProofRewriteRule
+
+/-- Produces a string representation. -/
+protected extern_def toString : ProofRewriteRule → String
+instance : ToString ProofRewriteRule := ⟨ProofRewriteRule.toString⟩
+
+/-- Produces a hash. -/
+extern_def hash : ProofRewriteRule → UInt64
+instance : Hashable ProofRewriteRule := ⟨ProofRewriteRule.hash⟩
+
+end ProofRewriteRule
+
+
+
+namespace UnknownExplanation
+
+/-- Produces a string representation. -/
+protected extern_def toString : UnknownExplanation → String
+instance : ToString UnknownExplanation := ⟨UnknownExplanation.toString⟩
+
+/-- Produces a hash. -/
+extern_def hash : UnknownExplanation → UInt64
+instance : Hashable UnknownExplanation := ⟨UnknownExplanation.hash⟩
+
+end UnknownExplanation
+
+namespace RoundingMode
+
+/-- Produces a string representation. -/
+protected extern_def toString : RoundingMode → String
+instance : ToString RoundingMode := ⟨RoundingMode.toString⟩
+
+/-- Produces a hash. -/
+extern_def hash : RoundingMode → UInt64
+instance : Hashable RoundingMode := ⟨RoundingMode.hash⟩
+
+end RoundingMode
+
+
+
+namespace BlockModelsMode
+
+/-- Produces a string representation. -/
+protected extern_def toString : BlockModelsMode → String
+instance : ToString BlockModelsMode := ⟨BlockModelsMode.toString⟩
+
+/-- Produces a hash. -/
+extern_def hash : BlockModelsMode → UInt64
+instance : Hashable BlockModelsMode := ⟨BlockModelsMode.hash⟩
+
+end BlockModelsMode
+
+
+
+namespace LearnedLitType
+
+/-- Produces a string representation. -/
+protected extern_def toString : LearnedLitType → String
+instance : ToString LearnedLitType := ⟨LearnedLitType.toString⟩
+
+/-- Produces a hash. -/
+extern_def hash : LearnedLitType → UInt64
+instance : Hashable LearnedLitType := ⟨LearnedLitType.hash⟩
+
+end LearnedLitType
+
+
+
+namespace ProofComponent
+
+/-- Produces a string representation. -/
+protected extern_def toString : ProofComponent → String
+instance : ToString ProofComponent := ⟨ProofComponent.toString⟩
+
+/-- Produces a hash. -/
+extern_def hash : ProofComponent → UInt64
+instance : Hashable ProofComponent := ⟨ProofComponent.hash⟩
+
+end ProofComponent
+
+
+
+namespace ProofFormat
+
+/-- Produces a string representation. -/
+protected extern_def toString : ProofFormat → String
+instance : ToString ProofFormat := ⟨ProofFormat.toString⟩
+
+/-- Produces a hash. -/
+extern_def hash : ProofFormat → UInt64
+instance : Hashable ProofFormat := ⟨ProofFormat.hash⟩
+
+end ProofFormat
+
+
+
+namespace FindSynthTarget
+
+/-- Produces a string representation. -/
+protected extern_def toString : FindSynthTarget → String
+instance : ToString FindSynthTarget := ⟨FindSynthTarget.toString⟩
+
+/-- Produces a hash. -/
+extern_def hash : FindSynthTarget → UInt64
+instance : Hashable FindSynthTarget := ⟨FindSynthTarget.hash⟩
+
+end FindSynthTarget
+
+
+
+namespace InputLanguage
+
+/-- Produces a string representation. -/
+protected extern_def toString : InputLanguage → String
+instance : ToString InputLanguage := ⟨InputLanguage.toString⟩
+
+/-- Produces a hash. -/
+extern_def hash : InputLanguage → UInt64
+instance : Hashable InputLanguage := ⟨InputLanguage.hash⟩
+
+end InputLanguage
+
+
+
+/-! ## Basic cvc5 types -/
+
+
+
+private opaque ResultImpl : NonemptyType.{0}
+
+/-- Encapsulation of a three-valued solver result, with explanations. -/
+def Result : Type := ResultImpl.type
+
+namespace Result
+
+instance : Nonempty Result := ResultImpl.property
+
+end Result
+
+
+
+private opaque SynthResultImpl : NonemptyType.{0}
+
+/-- Encapsulation of a three-valued solver result, with explanations. -/
+def SynthResult : Type := SynthResultImpl.type
+
+namespace SynthResult
+
+instance : Nonempty SynthResult := SynthResultImpl.property
+
+end SynthResult
+
+
+
+private opaque DatatypeConstructorDeclImpl : NonemptyType.{0}
+
+/-- A cvc5 datatype constructor declaration.
+
+A datatype constructor declaration is a specification used for creating a datatype constructor.
+-/
+def DatatypeConstructorDecl : Type := DatatypeConstructorDeclImpl.type
+
+namespace DatatypeConstructorDecl
+
+instance : Nonempty DatatypeConstructorDecl := DatatypeConstructorDeclImpl.property
+
+/-- A string representation of this datatype constructor declaration. -/
+protected extern_def toString : DatatypeConstructorDecl → String
+
+instance : ToString DatatypeConstructorDecl := ⟨DatatypeConstructorDecl.toString⟩
+
+end DatatypeConstructorDecl
+
+
+
+private opaque DatatypeDeclImpl : NonemptyType.{0}
+
+/-- A cvc5 datatype declaration.
+
+A datatype declaration is not itself a datatype (see `Datatype`), but a specification for creating a
+datatype sort.
+
+The interface for a datatype declaration coincides with the syntax for the SMT-LIB 2.6 command
+`declare-datatype`, or a single datatype within the `declare-datatypes` command.
+
+`Datatype` sorts can be constructed from a `DatatypeDecl` using:
+- `Solver.mkDatatypeSort`
+- `Solver.mkDatatypeSorts`
+-/
+def DatatypeDecl : Type := DatatypeDeclImpl.type
+
+namespace DatatypeDecl
+
+instance : Nonempty DatatypeDecl := DatatypeDeclImpl.property
+
+/-- Get a string representation of this datatype declaration. -/
+protected extern_def toString : DatatypeDecl → String
+
+instance : ToString DatatypeDecl := ⟨DatatypeDecl.toString⟩
+
+end DatatypeDecl
+
+
+
+private opaque DatatypeSelectorImpl : NonemptyType.{0}
+
+/-- A cvc5 datatype selector. -/
+def DatatypeSelector : Type := DatatypeSelectorImpl.type
+
+namespace DatatypeSelector
+
+instance : Nonempty DatatypeSelector := DatatypeSelectorImpl.property
+
+/-- Gte the string representation of this datatype selector. -/
+protected extern_def toString : DatatypeSelector → String
+
+instance : ToString DatatypeSelector := ⟨DatatypeSelector.toString⟩
+
+end DatatypeSelector
+
+
+
+private opaque DatatypeConstructorImpl : NonemptyType.{0}
+
+/-- A cvc5 datatype constructor. -/
+def DatatypeConstructor : Type := DatatypeConstructorImpl.type
+
+namespace DatatypeConstructor
+
+instance : Nonempty DatatypeConstructor := DatatypeConstructorImpl.property
+
+/-- A string representation of this datatype. -/
+protected extern_def toString : DatatypeConstructor → String
+
+instance : ToString DatatypeConstructor := ⟨DatatypeConstructor.toString⟩
+
+end DatatypeConstructor
+
+
+
+private opaque DatatypeImpl : NonemptyType.{0}
+
+/-- A cvc5 datatype. -/
+def Datatype : Type := DatatypeImpl.type
+
+namespace Datatype
+
+instance : Nonempty Datatype := DatatypeImpl.property
+
+/-- A string representation of this datatype. -/
+protected extern_def toString : Datatype → String
+
+instance : ToString Datatype := ⟨Datatype.toString⟩
+
+end Datatype
+
+
+
+private opaque GrammarImpl : NonemptyType.{0}
+
+/-- A Sygus Grammar.
+
+This class can be used to define a context-free grammar of terms. Its interface coincides with the
+definition of grammars in the SyGuS IF 2.1 standard.
+-/
+def Grammar : Type := GrammarImpl.type
+
+namespace Grammar
+
+instance : Nonempty Grammar := GrammarImpl.property
+
+/-- A string representation of this grammar. -/
+protected extern_def toString : Grammar → String
+
+instance : ToString Grammar := ⟨Grammar.toString⟩
+
+end Grammar
+
+
+
+private opaque CommandImpl : NonemptyType.{0}
+
+/-- Encapsulation of a command.
+
+Commands are constructed by the `InputParser` and can be invoked on the `Solver` and
+`Command`.
+-/
+def Command : Type := CommandImpl.type
+
+namespace Command
+
+instance : Nonempty Command := CommandImpl.property
+
+/-- Get a string representation of this command. -/
+protected extern_def toString : Command → String
+
+instance : ToString Command := ⟨Command.toString⟩
+
+end Command
