cvc5/Op.lean
@@ -1,0 +1,35 @@
+/-
+Copyright (c) 2023-2024 by the authors listed in the file AUTHORS and their
+institutional affiliations. All rights reserved.
+Released under Apache 2.0 license as described in the file LICENSE.
+Authors: Abdalrhman Mohamed, Adrien Champion
+-/
+
+
+
+import cvc5.Basic
+
+
+
+/-! # Operators -/
+namespace cvc5
+
+
+
+/-- Opaque operator type. -/
+private opaque OpImpl : NonemptyType.{0}
+
+/-- A cvc5 operator.
+
+An operator is a term that represents certain operators, instantiated with its required parameters,
+*e.g.*, a `Term` of kind `Kind.BITVECTOR_EXTRACT`.
+-/
+def Op : Type := OpImpl.type
+
+
+
+namespace Op
+
+instance : Nonempty Op := OpImpl.property
+
+end Op
