cvc5/Proof.lean
@@ -1,0 +1,34 @@
+/-
+Copyright (c) 2023-2024 by the authors listed in the file AUTHORS and their
+institutional affiliations. All rights reserved.
+Released under Apache 2.0 license as described in the file LICENSE.
+Authors: Abdalrhman Mohamed, Adrien Champion
+-/
+
+
+
+import cvc5.Basic
+
+
+
+/-! # Proofs -/
+namespace cvc5
+
+
+
+/-- Opaque proof type. -/
+private opaque ProofImpl : NonemptyType.{0}
+
+/-- A cvc5 proof.
+
+Proofs are trees and every proof object corresponds to the root step of a proof. The branches of the
+root step are the premises of the step.
+-/
+def Proof : Type := ProofImpl.type
+
+
+namespace Proof
+
+instance : Nonempty Proof := ProofImpl.property
+
+end Proof
