cvc5/Solver.lean
@@ -1,0 +1,13 @@
+/-
+Copyright (c) 2023-2024 by the authors listed in the file AUTHORS and their
+institutional affiliations. All rights reserved.
+Released under Apache 2.0 license as described in the file LICENSE.
+Authors: Abdalrhman Mohamed, Adrien Champion
+-/
+
+
+
+import cvc5.Basic
+import cvc5.Solver.Defs
+import cvc5.Solver.InputParser
+import cvc5.Solver.SymbolManager
