cvc5/Solver/Defs.lean
@@ -1,0 +1,36 @@
+/-
+Copyright (c) 2023-2024 by the authors listed in the file AUTHORS and their
+institutional affiliations. All rights reserved.
+Released under Apache 2.0 license as described in the file LICENSE.
+Authors: Abdalrhman Mohamed, Adrien Champion
+-/
+
+
+
+import cvc5.Basic
+
+
+
+
+/-! # Solver -/
+namespace cvc5
+
+
+
+/-- Opaque solver type. -/
+private opaque SolverImpl : NonemptyType.{0}
+
+/-- A cvc5 solver. -/
+def Solver : Type := SolverImpl.type
+
+namespace Solver
+
+instance : Nonempty Solver := SolverImpl.property
+
+/-- Constructor.
+
+- `tm` The associated term manager instance.
+-/
+extern_def new : (tm : TermManager) → Env Solver
+
+end Solver
