cvc5/Solver/InputParser.lean
@@ -1,0 +1,71 @@
+/-
+Copyright (c) 2023-2024 by the authors listed in the file AUTHORS and their
+institutional affiliations. All rights reserved.
+Released under Apache 2.0 license as described in the file LICENSE.
+Authors: Abdalrhman Mohamed, Adrien Champion
+-/
+
+
+
+import cvc5.Basic
+import cvc5.Solver.Defs
+import cvc5.Solver.SymbolManager
+
+
+
+/-! # Operators -/
+namespace cvc5
+
+
+
+/-- Opaque operator type. -/
+private opaque InputParserImpl : NonemptyType.{0}
+
+/-- This type is the main interface for retrieving commands and expressions from an input using a
+  parser.
+
+After construction, it is expected that an input is first configured via, e.g.,
+`InputParser.setFileInput`, `InputParser.setStreamInput`, `InputParser.setStringInput` or
+`InputParser.setIncrementalStringInput` and `InputParser.appendIncrementalStringInput`. Then,
+functions `InputParser.nextCommand` and `InputParser.nextExpression` can be invoked to parse the
+input.
+
+The input parser interacts with a symbol manager, which determines which symbols are defined in the
+current context, based on the background logic and user-defined symbols. If no symbol manager is
+provided, then the input parser will construct (an initially empty) one.
+
+If provided, the symbol manager must have a logic that is compatible with the provided solver. That
+is, if both the solver and symbol manager have their logics set (`SymbolManager.isLogicSet` and
+`Solver.isLogicSet`), then their logics must be the same.
+
+Upon setting an input source, if either the solver (resp. symbol manager) has its logic set, then
+the symbol manager (resp. solver) is set to use that logic, if its logic is not already set.
+-/
+def InputParser : Type := InputParserImpl.type
+
+
+
+namespace InputParser
+
+instance : Nonempty InputParser := InputParserImpl.property
+
+/-- Construct an input parser with an initially empty symbol manager.
+
+- `solver`: The solver (e.g. for constructing terms and sorts).
+-/
+private extern_def ofSolver : (solver : Solver) → Env InputParser
+
+/-- Construct an input parser.
+
+- `solver` The solver (e.g. for constructing terms and sorts).
+- `sm` The symbol manager, which contains a symbol table that maps symbols to terms and sorts. Must
+  have a logic that is compatible with the solver.
+-/
+private extern_def ofSolverAndSM : (solver : Solver) → (sm : SymbolManager) → Env InputParser
+
+@[inherit_doc ofSolverAndSM]
+def new (solver : Solver) : (sm : Option SymbolManager := none) → Env InputParser
+  | none => ofSolver solver
+  | some sm => ofSolverAndSM solver sm
+
+end InputParser
