cvc5/Solver/SymbolManager.lean
@@ -1,0 +1,49 @@
+/-
+Copyright (c) 2023-2024 by the authors listed in the file AUTHORS and their
+institutional affiliations. All rights reserved.
+Released under Apache 2.0 license as described in the file LICENSE.
+Authors: Abdalrhman Mohamed, Adrien Champion
+-/
+
+
+
+import cvc5.Basic
+import cvc5.TermManager
+
+
+
+/-! # Symbol manager -/
+namespace cvc5
+
+
+
+/-- Opaque symbol manager type. -/
+private opaque SymbolManagerImpl : NonemptyType.{0}
+
+/-- Symbol manager.
+
+Internally, this class manages a symbol table and other meta-information pertaining to SMT2 file
+inputs (*e.g.* named assertions, declared functions, *etc.*).
+
+A symbol manager can be modified by invoking commands, see `Command.invoke`.
+
+A symbol manager can be provided when constructing an `InputParser`, in which case that
+`InputParser` has symbols of this symbol manager preloaded.
+
+The symbol manager's interface is otherwise not publicly available.
+-/
+def SymbolManager : Type := SymbolManagerImpl.type
+
+
+
+namespace SymbolManager
+
+instance : Nonempty SymbolManager := SymbolManagerImpl.property
+
+/-- Constructor.
+
+- `tm` The associated term manager instance.
+-/
+extern_def new : (tm : TermManager) → Env SymbolManager
+
+end SymbolManager
