cvc5/Sort.lean
@@ -1,0 +1,31 @@
+/-
+Copyright (c) 2023-2024 by the authors listed in the file AUTHORS and their
+institutional affiliations. All rights reserved.
+Released under Apache 2.0 license as described in the file LICENSE.
+Authors: Abdalrhman Mohamed, Adrien Champion
+-/
+
+
+
+import cvc5.Basic
+
+
+
+/-! # Sorts -/
+namespace cvc5
+
+
+
+/-- Opaque sort type. -/
+private opaque SortImpl : NonemptyType.{0}
+
+/-- The sort of a cvc5 term. -/
+def «Sort» : Type := cvc5.SortImpl.type
+
+
+
+namespace «Sort»
+
+instance : Nonempty cvc5.Sort := SortImpl.property
+
+end «Sort»
