cvc5/Term.lean
@@ -1,0 +1,31 @@
+/-
+Copyright (c) 2023-2024 by the authors listed in the file AUTHORS and their
+institutional affiliations. All rights reserved.
+Released under Apache 2.0 license as described in the file LICENSE.
+Authors: Abdalrhman Mohamed, Adrien Champion
+-/
+
+
+
+import cvc5.Basic
+
+
+
+/-! # Terms -/
+namespace cvc5
+
+
+
+/-- Opaque term type. -/
+private opaque TermImpl : NonemptyType.{0}
+
+/-- A cvc5 term. -/
+def Term : Type := TermImpl.type
+
+
+
+namespace Term
+
+instance : Nonempty Term := TermImpl.property
+
+end Term
