cvc5/TermManager.lean
@@ -1,0 +1,34 @@
+/-
+Copyright (c) 2023-2024 by the authors listed in the file AUTHORS and their
+institutional affiliations. All rights reserved.
+Released under Apache 2.0 license as described in the file LICENSE.
+Authors: Abdalrhman Mohamed, Adrien Champion
+-/
+
+
+
+import cvc5.Basic
+
+
+
+/-! # Term manager -/
+namespace cvc5
+
+
+
+/-- Opaque term manager type. -/
+private opaque TermManagerImpl : NonemptyType.{0}
+
+/-- Manager for cvc5 terms. -/
+def TermManager : Type := TermManagerImpl.type
+
+
+
+namespace TermManager
+
+instance : Nonempty TermManager := TermManagerImpl.property
+
+/-- Constructor. -/
+extern_def new : Env TermManager
+
+end TermManager
